vrefinedep WIP 1/n

src/Slabs.fst
@@ -723,8 +723,236 @@ let alloc_metadata
   return r
 #pop-options
 
+let p1 (v: U32.t) : prop
+  = (U32.v v < U32.v metadata_max) == true
+
+let p2 (v: U32.t) : prop
+  = (U32.v v <= U32.v metadata_max) == true
+
+assume val vrefinedep_hp
+  (v: vprop)
+  (p: ( (t_of v) -> Tot prop))
+  (f: ( (x:t_of v{p x}) -> Tot vprop))
+  : Tot (SM.slprop u#1)
+
+[@__steel_reduce__]
+let vrefinedep_t
+  (v: vprop)
+  (p: ( (t_of v) -> Tot prop))
+  (f: ( (x:t_of v{p x}) -> Tot vprop))
+  : Tot Type
+  =
+  dtuple2 (x: (t_of v){p x}) (fun x -> t_of (f x))
+
+assume val vrefinedep_sel
+  (v: vprop)
+  (p: ( normal (t_of v) -> Tot prop))
+  (f: ( normal (x:t_of v{p x}) -> Tot vprop))
+  : Tot (selector (vrefinedep_t v p f) (vrefinedep_hp v p f))
+
+[@@__steel_reduce__]
+let vrefinedep'
+  (v: vprop)
+  (p: ( normal (t_of v) -> Tot prop))
+  (f: ( normal (x:t_of v{p x}) -> Tot vprop))
+  : Tot vprop' = {
+  hp = vrefinedep_hp v p f;
+  t = vrefinedep_t v p f;
+  sel = vrefinedep_sel v p f;
+}
+[@@__steel_reduce__]
+let vrefinedep
+  (v: vprop)
+  (p: ( normal (t_of v) -> Tot prop))
+  (f: ( normal (x:t_of v{p x}) -> Tot vprop))
+  = VUnit (vrefinedep' v p f)
+
+assume val elim_vrefinedep (#opened:_)
+  (v: vprop)
+  (p: ( normal (t_of v) -> Tot prop))
+  (f: ( normal (x:t_of v{p x}) -> Tot vprop))
+  : SteelGhost (G.erased (x: normal (t_of v){p x})) opened
+  (vrefine v p `vdep` f)
+  (fun res -> v `star` f (G.reveal res))
+  (requires fun _ -> True)
+  (ensures fun h res h' ->
+    p res /\
+    G.reveal res == h' v /\
+    (let fs : x:t_of v{p x} = h' v in
+    let sn : t_of (f (G.reveal res)) = h' (f (G.reveal res)) in
+    let x2 = h (vrefine v p `vdep` f) in
+    G.reveal res == fs /\
+    dfst x2 == fs /\
+    dsnd x2 == sn /\
+    True)
+  )
+
+assume val intro_vrefinedep (#opened:_)
+  (v: vprop)
+  (p: ( normal (t_of v) -> Tot prop))
+  (f': vprop)
+  (f: ( normal (x:t_of v{p x}) -> Tot vprop))
+  : SteelGhost unit opened
+  (v `star` f')
+  (fun _ -> vrefine v p `vdep` f)
+  (requires fun h ->
+    p (h v) /\
+    f' == f (h v))
+  (ensures fun h _ h' ->
+    p (h v) /\
+    f' == f (h v) /\
+    (let x2 = h' (vrefine v p `vdep` f) in
+    let sn : t_of f' = h f' in
+    dfst x2 == h v /\
+    dsnd x2 == sn)
+  )
+
+let vrefinedep_idem (#opened:_)
+  (v: vprop)
+  (p: ( normal (t_of v) -> Tot prop))
+  (f: ( normal (x:t_of v{p x}) -> Tot vprop))
+  : SteelGhost unit opened
+  (vrefine v p `vdep` f)
+  (fun _ -> vrefine v p `vdep` f)
+  (requires fun _ -> True)
+  (ensures fun h _ h' ->
+    h (vrefine v p `vdep` f)
+    ==
+    h' (vrefine v p `vdep` f)
+  )
+  =
+  let x = elim_vrefinedep v p f in
+  intro_vrefinedep v p (f (G.reveal x)) f
+
+let alloc_metadata2
+  (size_class: sc)
+  (slab_region: array U8.t{A.length slab_region = U32.v metadata_max * U32.v page_size})
+  (md_bm_region: array U64.t{A.length md_bm_region = U32.v metadata_max * 4})
+  (md_region: array (SL.cell blob){A.length md_region = U32.v metadata_max})
+  (md_count: ref U32.t)
+  //: Steel (SL.t blob)
+  : Steel unit
+  (
+    vptr md_count
+      `vrefine`
+      p1
+      `vdep`
+      (fun (v: U32.t{U32.v v < U32.v metadata_max}) ->
+        A.varray (A.split_r slab_region (u32_to_sz (U32.mul v page_size))) `star`
+        A.varray (A.split_r md_bm_region (u32_to_sz (U32.mul v 4ul))) `star`
+        A.varray (A.split_r md_region (u32_to_sz v))
+    )
+  )
+  (fun r ->
+    //SL.llist (p_empty size_class) r `star`
+    (vptr md_count
+      `vrefine`
+      p1
+      `vdep`
+      (fun (v: U32.t{U32.v v < U32.v metadata_max}) ->
+        A.varray (A.split_r slab_region (u32_to_sz (U32.mul v page_size))) `star`
+        A.varray (A.split_r md_bm_region (u32_to_sz (U32.mul v 4ul))) `star`
+        A.varray (A.split_r md_region (u32_to_sz v))
+    ))
+  )
+  (requires fun h0 -> True
+    //sel md_count h0 = G.reveal md_count_v
+  )
+  (ensures fun h0 r h1 ->
+    //L.length (SL.v_llist (p_empty size_class) r h1) = 1 /\
+    True
+    //sel md_count h1 = U32.add (sel md_count h0) 1ul
+  )
+  =
+  let x = elim_vrefinedep
+    (vptr md_count)
+    (fun x -> U32.v x < U32.v metadata_max)
+    (fun v ->
+      A.varray (A.split_r slab_region (u32_to_sz (U32.mul v page_size))) `star`
+      A.varray (A.split_r md_bm_region (u32_to_sz (U32.mul v 4ul))) `star`
+      A.varray (A.split_r md_region (u32_to_sz v))
+    )
+  in
+  sladmit ();
+  return ()
 
 
+
+let a  =42
+
+(*)
+
+  let v0 : G.erased (v:U32.t{U32.v v < U32.v metadata_max}) = gget (
+    vptr md_count
+      `vrefine`
+      p1
+      `vdep`
+      (fun (v: U32.t{U32.v v < U32.v metadata_max}) ->
+        A.varray (A.split_r slab_region (u32_to_sz (U32.mul v page_size))) `star`
+        A.varray (A.split_r md_bm_region (u32_to_sz (U32.mul v 4ul))) `star`
+        A.varray (A.split_r md_region (u32_to_sz v))
+    )
+  ) in
+  assert (U32.v (G.reveal v0) < U32.v metadata_max);
+
+
+  return ()
+
+
+let a = 42
+
+(*)
+  (
+    vptr md_count `star`
+    A.varray (A.split_r slab_region (u32_to_sz (U32.mul (G.reveal md_count_v) page_size))) `star`
+    A.varray (A.split_r md_bm_region (u32_to_sz (U32.mul (G.reveal md_count_v) 4ul))) `star`
+    A.varray (A.split_r md_region (u32_to_sz (G.reveal md_count_v)))
+  )
+
+
+  
+
+
+
+
+assume val alloc_metadata2
+  (size_class: sc)
+  (slab_region: array U8.t{A.length slab_region = U32.v metadata_max * U32.v page_size})
+  (md_bm_region: array U64.t{A.length md_bm_region = U32.v metadata_max * 4})
+  (md_region: array (SL.cell blob){A.length md_region = U32.v metadata_max})
+  (md_count: ref U32.t)
+  : Steel (SL.t blob)
+  (
+    vptr md_count
+      `vrefine`
+      p1
+      `vdep`
+      (fun (v: U32.t{U32.v v < U32.v metadata_max}) ->
+        A.varray (A.split_r slab_region (u32_to_sz (U32.mul v page_size))) `star`
+        A.varray (A.split_r md_bm_region (u32_to_sz (U32.mul v 4ul))) `star`
+        A.varray (A.split_r md_region (u32_to_sz v))
+    )
+  )
+  (fun r ->
+    SL.llist (p_empty size_class) r `star`
+    (vptr md_count
+      `vrefine`
+      p2
+      `vdep`
+      (fun (v: U32.t{U32.v v <= U32.v metadata_max}) ->
+        A.varray (A.split_r slab_region (u32_to_sz (U32.mul v page_size))) `star`
+        A.varray (A.split_r md_bm_region (u32_to_sz (U32.mul v 4ul))) `star`
+        A.varray (A.split_r md_region (u32_to_sz v))
+    ))
+  )
+  (requires fun h0 -> True
+    //sel md_count h0 = G.reveal md_count_v
+  )
+  (ensures fun h0 r h1 ->
+    L.length (SL.v_llist (p_empty size_class) r h1) = 1 /\
+    True
+    //sel md_count h1 = U32.add (sel md_count h0) 1ul
+  )
 
 
 let unpack_list_singleton (#a: Type0)
